Use structured names.
This replaces the entire AST with structured names and ports the logic and
infrastructure.

Also,

- Work around storing [SourceLocation] in [Loc].
Other compilers support this, but it seems that what we build with
in CI does not.

src/PrePrint.cpp
@@ -173,6 +173,7 @@ struct PrePrint :
 		Visit(decl->getType());
 	}
 	void VisitFunctionDecl(const FunctionDecl* decl) {
+		VisitName(decl);
 		if (decl->getBody())
 			Visit(decl->getBody());
 		for (auto i : decl->parameters()) {
@@ -181,11 +182,13 @@ struct PrePrint :
 		Visit(decl->getReturnType());
 	}
 	void VisitCXXConstructorDecl(const CXXConstructorDecl* decl) {
+		VisitName(decl);
 		for (auto i : decl->inits())
 			Visit(i->getInit());
 		VisitFunctionDecl(decl);
 	}
-	void VisitCXXRecordDecl(const CXXRecordDecl* decl) {
+	void VisitRecordDecl(const RecordDecl* decl) {
+		VisitName(decl);
 		for (auto i : decl->fields()) {
 			Visit(i->getType());
 		}
