theories/lang/cpp/syntax/types.v
@@ -7,557 +7,13 @@ Require Import bedrock.prelude.elpi.derive.
 Require Import bedrock.prelude.base.
 Require Import bedrock.prelude.bool.
 Require Import bedrock.prelude.list.
-Require Export bedrock.lang.cpp.arith.types.
-Require Import bedrock.lang.cpp.syntax.names.
+Require Export bedrock.lang.cpp.syntax.core.
 
 Set Primitive Projections.
 
-(* Type qualifiers *)
-Variant type_qualifiers : Set :=
-| QCV (* const volatile *)
-| QC (* const *)
-| QV (* volatile *)
-| QM (* no qualifiers *)
-.
-#[only(inhabited,eq_dec,countable)] derive type_qualifiers.
-
-Definition q_const (q : type_qualifiers) : bool :=
-  match q with
-  | QCV | QC => true
-  | _ => false
-  end.
-Definition q_volatile (q : type_qualifiers) : bool :=
-  match q with
-  | QCV | QV => true
-  | _ => false
-  end.
-Definition CV (const volatile : bool) :=
-  match const , volatile with
-  | true , true => QCV
-  | true , false => QC
-  | false , true => QV
-  | false , false => QM
-  end.
-
-(* [merge_tq a b] computes the join of the restrictions of [a] and [b],
-   i.e. if either [a] or [b] is const/volatile, the result will be const/volatile.
-   This is used to compress adjacent qualifiers.
- *)
-Definition merge_tq (a b : type_qualifiers) : type_qualifiers :=
-  CV (q_const a || q_const b) (q_volatile a || q_volatile b).
-
-#[global] Instance merge_tq_idemp : IdemP (=) merge_tq.
-Proof. by intros []. Qed.
-#[global] Instance merge_tq_left_id : LeftId (=) QM merge_tq.
-Proof. by intros []. Qed.
-#[global] Instance merge_tq_right_id : RightId (=) QM merge_tq.
-Proof. by intros []. Qed.
-#[global] Instance merge_tq_left_absorb : LeftAbsorb (=) QCV merge_tq.
-Proof. by intros []. Qed.
-#[global] Instance merge_tq_right_absorb : RightAbsorb (=) QCV merge_tq.
-Proof. by intros []. Qed.
-#[global] Instance merge_tq_comm : Comm (=) merge_tq.
-Proof. by intros [] []. Qed.
-#[global] Instance merge_tq_assoc : Assoc (=) merge_tq.
-Proof. by intros [] [] []. Qed.
-
-Lemma merge_tq_QM_inj q1 q2 : merge_tq q1 q2 = QM -> q1 = QM /\ q2 = QM.
-Proof. destruct q1, q2; naive_solver. Qed.
-
-(**
-The preorder from
-<https://eel.is/c++draft/basic.type.qualifier#5>
-*)
-Definition tq_le (a b : type_qualifiers) : Prop :=
-  ∃ c, b = merge_tq a c.
-
-Definition is_tq_le (a b : type_qualifiers) : bool :=
-  bool_decide (a = b) ||
-  match a , b with
-  | QM , _ => true
-  | QC , QCV => true
-  | QV , QCV => true
-  | _, _ => false
-  end.
-
-Lemma tq_le_is_tq_le a b : tq_le a b <-> is_tq_le a b.
-Proof.
-  split.
-  { intros (c & ->). by destruct a, c. }
-  { rewrite /is_tq_le=>?. case_bool_decide.
-    - subst a. exists QM. by destruct b.
-    - destruct a, b; first [ done | by exists QV | by exists QC | by exists QCV ]. }
-Qed.
-
-#[global] Instance tq_le_dec : RelDecision tq_le.
-Proof.
-  refine (fun a b => cast_if (decide (is_tq_le a b))).
-  all: abstract (by rewrite tq_le_is_tq_le).
-Defined.
-
-(* Calling conventions are a little bit beyond what is formally blessed by
-   C++, but the are necessary for low level code that links with other
-   languages.
-
-   From the C++ standard point of view, we view these as opaque symbols with
-   no particular meaning. All that matters is that when you call a function,
-   that this calling convention matches between the caller and the callee.
-   This is what ensures, for example, that when you call a function implemented
-   in another language, that you have the appropriate annotations in place.
-   For example, if you were calling an OpenCL kernel, then the function would
-   have type [Tfunction (cc:=CC_OpenCLKernel) ..], and you would require that
-   annotation in your program.
- *)
-Variant calling_conv : Set :=
-| CC_C
-| CC_MsAbi
-| CC_RegCall.
-#[only(inhabited,eq_dec,countable)] derive calling_conv.
-
-(* in almost all contexts, we are going to use [CC_C], so we're going to make
-   that the default. Clients interested in specifying another calling convention
-   should write, e.g., [Tfunction (cc:=CC_RegCall) ..] to specify the
-   calling convention explicitly.
- *)
-Existing Class calling_conv.
-#[global] Existing Instance CC_C.
-
-Variant function_arity : Set :=
-| Ar_Definite
-| Ar_Variadic.
-#[only(inhabited,eq_dec,countable)] derive function_arity.
-
-(* In almost all contexts, we will use [Ar_Definite], so that is the default. *)
-Existing Class function_arity.
-#[global] Existing Instance Ar_Definite.
-
-(** Character types
-    See https://en.cppreference.com/w/cpp/language/types
- *)
-Module char_type.
-  Variant t : Set :=
-    | Cchar (* signedness defined by platform *)
-    | Cwchar (* signedness defined by platform *)
-    | C8 (* unsigned *)
-    | C16 (* unsigned *)
-    | C32. (* unsigned *)
-  #[global] Instance t_eq_dec: EqDecision t.
-  Proof. solve_decision. Defined.
-  #[global] Instance t_countable : Countable t.
-  Proof.
-    apply (inj_countable'
-      (λ cc,
-        match cc with
-        | Cchar => 0 | Cwchar => 1 | C8 => 2 | C16 => 3 | C32 => 4
-        end)
-      (λ n,
-        match n with
-        | 0 => Cchar | 1 => Cwchar | 2 => C8 | 3 => C16 | 4 => C32
-        | _ => Cchar	(** dummy *)
-        end)).
-    abstract (by intros []).
-  Defined.
-
-  Definition bytesN (t : t) : N :=
-    match t with
-    | Cchar => 1
-    | Cwchar => 4 (* TODO: actually 16-bits on Windows *)
-    | C8 => 1
-    | C16 => 2
-    | C32 => 4
-    end.
-  #[global] Arguments bytesN !_ /.
-
-  Definition bitsN (t : t) : N :=
-    8 * bytesN t.
-  #[global] Arguments bitsN !_ /.
-
-End char_type.
-Notation char_type := char_type.t.
-
-(** Integer types
-    See https://en.cppreference.com/w/cpp/language/types
- *)
-Module int_type.
-  (* the rank <https://eel.is/c++draft/conv.rank> *)
-  Notation t := bitsize (only parsing).
-  Notation rank := t (only parsing).
-
-  Notation Ichar := W8 (only parsing).
-  Notation Ishort := W16 (only parsing).
-  Notation Iint := W32 (only parsing).
-  Notation Ilong := W64 (only parsing).
-  (** warning: LLP64 model uses [long_bits := W32] *)
-  Notation Ilonglong := W64 (only parsing).
-
-  Definition bytesN (t : t) : N :=
-    arith.types.bytesN t. (* from [arith.types] *)
-
-  Definition bitsN (t : t) : N :=
-    8 * bytesN t.
-
-  Definition t_le (a b : t) : Prop :=
-    (bytesN a <= bytesN b)%N.
-
-  #[global] Instance t_le_dec : RelDecision t_le :=
-    fun a b => N.le_dec (bytesN a) (bytesN b).
-
-  (* [max] on the rank. *)
-  Definition t_max (a b : bitsize) : bitsize :=
-    if bool_decide (t_le a b) then b else a.
-
-End int_type.
-Notation int_type := int_type.t.
-
-Module float_type.
-  Variant t : Set :=
-    | Ffloat16
-    | Ffloat
-    | Fdouble
-    | Flongdouble
-    | Ffloat128.
-
-  #[global] Instance t_eq_dec : EqDecision t := ltac:(solve_decision).
-  #[global] Instance t_countable : Countable t.
-  Proof.
-    apply (inj_countable'
-      (λ cc,
-        match cc with
-        | Ffloat16 => 3 | Ffloat => 0 | Fdouble => 1 | Flongdouble => 2 | Ffloat128 => 4
-        end)
-      (λ n,
-        match n with
-        | 0 => Ffloat | 1 => Fdouble | 2 => Flongdouble | 3 => Ffloat16 | 4 => Ffloat128
-        | _ => Ffloat	(** dummy *)
-        end)).
-    abstract (by intros []).
-  Defined.
-
-  Definition bytesN (t : t) : N :=
-    match t with
-    | Ffloat16 => 2
-    | Ffloat => 4
-    | Fdouble => 8
-    | Flongdouble => 16
-    | Ffloat128 => Evaluate (128 / 8)%N
-    end.
-
-  Definition bitsN (t : t) : N :=
-    8 * bytesN t.
-
-End float_type.
-
-(* types *)
-Inductive type : Set :=
-| Tptr (_ : (*expr*)type)
-| Tref (_ : (*expr*)type)
-| Trv_ref (_ : (*expr*)type)
-  (**
-  Note: cpp2v (really, clang's parser) handles so-called "reference
-  collapsing": We do not see references to references.
-
-  Background:
-  https://en.cppreference.com/w/cpp/language/reference#Reference_collapsing
-  https://www.eel.is/c++draft/dcl.ref#5
-  *)
-| Tnum (size : int_type.t) (signed : signed)
-| Tchar_ (_ : char_type)
-| Tvoid
-| Tarray (_ : type) (_ : N)
-| Tincomplete_array (_ : type)
-| Tvariable_array (_ : type) (* (_ : Expr) -- not supported *)
-| Tnamed (_ : globname)
-| Tenum (_ : globname) (* enumerations *)
-| Tfunction {cc : calling_conv} {ar : function_arity} (_ : (*decl*)type) (_ : list (*decl*)type)
-| Tbool
-| Tmember_pointer (_ : globname) (_ : (*expr*)type)
-| Tfloat_ (_ : float_type.t)
-| Tqualified (_ : type_qualifiers) (_ : type)
-| Tnullptr
-(* architecture-specific types; currently unused.
-   some [Tarch] types, e.g. ARM SVE, are "sizeless", hence [option size]. *)
-| Tarch (_ : option bitsize) (name : bs)
-| Tunsupported (_ : bs)
-.
-(**
-For documentation purposes, we often use the following aliases.
-
-- [decltype] _declaration types_ arise in variable declarations
-(including function arguments)
-
-- [exprtype] _expression types_ are assigned to expressions
-(together with value categories) by the static semantics of C++
-
-- [functype] _function types_ are known to be [Tfunction]
-
-Roughly, we have an isomorphism [decltype ≅ exprtype × ValCat]. While
-variables can be declared with reference types, expressions never have
-reference types (that information being present in the expression's
-value category).
-*)
-Definition decltype : Set := type.
-Definition exprtype : Set := type.
-Definition functype : Set := type.
-
-#[only(inhabited)] derive type.
-
-(** Strengthened Induction Principle for [type]
-
-    [type] is a `Nested Inductive Type` due to the use of [list type]
-    in the [Tfunction] constructor. In Coq, the default induction
-    principle generated for a nested inductive type is too weak because
-    it fails to thread the indexed predicate through the structure
-    of the parameterized type family. While strengthened induction
-    principles are not generally derivable, we can manually strengthen
-    it if we can find a way to incorporate the nested uses of the Type.
-    Luckily, we can use [List.Forall] to express that the indexed
-    predicate must hold on each element of the list which is sufficient
-    for the [normalize_type_idempotent] Lemma. For more information on
-    this topic, please refer to [1].
-
-    [1] http://adam.chlipala.net/cpdt/html/InductiveTypes.html;
-          "Nested Inductive Types" Section
- *)
-Section type_ind'.
-  Variable P : type -> Prop.
-
-  Hypothesis Tptr_ind' : forall (ty : type),
-    P ty -> P (Tptr ty).
-  Hypothesis Tref_ind' : forall (ty : type),
-    P ty -> P (Tref ty).
-  Hypothesis Trv_ref_ind' : forall (ty : type),
-    P ty -> P (Trv_ref ty).
-  Hypothesis Tnum_ind' : forall (size : bitsize) (sign : signed),
-    P (Tnum size sign).
-  Hypothesis Tchar__ind' : forall ct, P (Tchar_ ct).
-  Hypothesis Tvoid_ind' : P Tvoid.
-  Hypothesis Tarray_ind' : forall (ty : type) (sz : N),
-    P ty -> P (Tarray ty sz).
-  Hypothesis Tincomplete_array_ind' : forall ty,
-    P ty -> P (Tincomplete_array ty).
-  Hypothesis Tvariable_array_ind' : forall ty,
-    P ty -> P (Tvariable_array ty).
-  Hypothesis Tnamed_ind' : forall (name : globname),
-    P (Tnamed name).
-  Hypothesis Tenum_ind' : forall (name : globname),
-    P (Tenum name).
-  Hypothesis Tfunction_ind' : forall {cc : calling_conv} {ar : function_arity} (ty : type) (tys : list type),
-    P ty -> Forall P tys -> P (Tfunction ty tys).
-  Hypothesis Tbool_ind' : P Tbool.
-  Hypothesis Tmember_pointer_ind' : forall (name : globname) (ty : type),
-    P ty -> P (Tmember_pointer name ty).
-  Hypothesis Tfloat_ind' : forall (size : float_type.t),
-    P (Tfloat_ size).
-  Hypothesis Tqualified_ind' : forall (q : type_qualifiers) (ty : type),
-    P ty -> P (Tqualified q ty).
-  Hypothesis Tnullptr_ind' : P Tnullptr.
-  Hypothesis Tarch_ind' : forall (osize : option bitsize) (name : bs),
-    P (Tarch osize name).
-  Hypothesis Tunsupported' : forall (msg : bs),
-    P (Tunsupported msg).
-
-  Fixpoint type_ind' (ty : type) : P ty :=
-    match ty with
-    | Tptr ty                 => Tptr_ind' ty (type_ind' ty)
-    | Tref ty                 => Tref_ind' ty (type_ind' ty)
-    | Trv_ref ty              => Trv_ref_ind' ty (type_ind' ty)
-    | Tnum sz sgn             => Tnum_ind' sz sgn
-    | Tchar_ sz               => Tchar__ind' sz
-    | Tvoid                   => Tvoid_ind'
-    | Tarray ty sz            => Tarray_ind' ty sz (type_ind' ty)
-    | Tincomplete_array ty    => Tincomplete_array_ind' ty (type_ind' ty)
-    | Tvariable_array ty      => Tvariable_array_ind' ty (type_ind' ty)
-    | Tnamed name             => Tnamed_ind' name
-    | Tenum name              => Tenum_ind' name
-    | Tfunction ty tys        =>
-      Tfunction_ind' ty tys (type_ind' ty)
-                     (* NOTE: We must use a nested [fix] in order to convince Coq that
-                          the elements of [tys] are actually subterms of
-                          [Tfunction ty tys]
-                      *)
-                     ((fix list_tys_ind' (tys : list type) : Forall P tys :=
-                         match tys with
-                         | []        => List.Forall_nil P
-                         | ty :: tys' => List.Forall_cons P ty tys'
-                                                        (type_ind' ty) (list_tys_ind' tys')
-                         end) tys)
-    | Tbool                   => Tbool_ind'
-    | Tmember_pointer name ty => Tmember_pointer_ind' name ty (type_ind' ty)
-    | Tfloat_ sz               => Tfloat_ind' sz
-    | Tqualified q ty         => Tqualified_ind' q ty (type_ind' ty)
-    | Tnullptr                => Tnullptr_ind'
-    | Tarch osize name        => Tarch_ind' osize name
-    | Tunsupported msg        => Tunsupported' msg
-    end.
-End type_ind'.
-
-(* XXX merge type_eq_dec into type_eq. *)
-Definition type_eq_dec : forall (ty1 ty2 : type), { ty1 = ty2 } + { ty1 <> ty2 }.
-Proof.
-  (* rewrite /RelDecision /Decision. *)
-  fix IHty1 1.
-  rewrite -{1}/(EqDecision type) in IHty1.
-  decide equality; try solve_trivial_decision.
-Defined.
-#[global] Instance type_eq: EqDecision type := type_eq_dec.
-Section type_countable.
-  #[local] Notation BS x        := (GenLeaf (inr x)).
-  #[local] Notation QUAL x      := (GenLeaf (inl (inr x))).
-  #[local] Notation BITSIZE x   := (GenLeaf (inl (inl (inr x)))).
-  #[local] Notation SIGNED x    := (GenLeaf (inl (inl (inl (inr x))))).
-  #[local] Notation CC x        := (GenLeaf (inl (inl (inl (inl (inr x)))))).
-  #[local] Notation AR x        := (GenLeaf (inl (inl (inl (inl (inl (inr x))))))).
-  #[local] Notation N x         := (GenLeaf (inl (inl (inl (inl (inl (inl (inr x)))))))).
-  #[local] Notation CHAR_TYPE x := (GenLeaf (inl (inl (inl (inl (inl (inl (inl (inr x))))))))).
-  #[local] Notation FLOAT_TYPE x := (GenLeaf (inl (inl (inl (inl (inl (inl (inl (inl x))))))))).
-
-  #[global] Instance type_countable : Countable type.
-  Proof.
-    set enc := fix go (t : type) :=
-      match t with
-      | Tptr t => GenNode 0 [go t]
-      | Tref t => GenNode 1 [go t]
-      | Trv_ref t => GenNode 2 [go t]
-      | Tnum sz sgn => GenNode 3 [BITSIZE sz; SIGNED sgn]
-      | Tvoid => GenNode 4 []
-      | Tarray t n => GenNode 5 [go t; N n]
-      | Tincomplete_array t => GenNode 17 [go t]
-      | Tvariable_array t => GenNode 18 [go t]
-      | Tnamed gn => GenNode 6 [BS gn]
-      | @Tfunction cc ar ret args => GenNode 7 $ (CC cc) :: (AR ar) :: go ret :: (go <$> args)
-      | Tbool => GenNode 8 []
-      | Tmember_pointer gn t => GenNode 9 [BS gn; go t]
-      | Tfloat_ sz => GenNode 10 [FLOAT_TYPE sz]
-      | Tqualified q t => GenNode 11 [QUAL q; go t]
-      | Tnullptr => GenNode 12 []
-      | Tarch None gn => GenNode 13 [BS gn]
-      | Tarch (Some sz) gn => GenNode 14 [BITSIZE sz; BS gn]
-      | Tenum gn => GenNode 15 [BS gn]
-      | Tchar_ sz => GenNode 16 [CHAR_TYPE sz]
-      | Tunsupported msg => GenNode 19 [BS msg]
-      end.
-    set dec := fix go t :=
-      match t with
-      | GenNode 0 [t] => Tptr (go t)
-      | GenNode 1 [t] => Tref (go t)
-      | GenNode 2 [t] => Trv_ref (go t)
-      | GenNode 3 [BITSIZE sz; SIGNED sgn] => Tnum sz sgn
-      | GenNode 4 [] => Tvoid
-      | GenNode 5 [t; N n] => Tarray (go t) n
-      | GenNode 17 [t] => Tincomplete_array (go t)
-      | GenNode 18 [t] => Tvariable_array (go t)
-      | GenNode 6 [BS gn] => Tnamed gn
-      | GenNode 7 (CC cc :: AR ar :: ret :: args) => @Tfunction cc ar (go ret) (go <$> args)
-      | GenNode 8 [] => Tbool
-      | GenNode 9 [BS gn; t] => Tmember_pointer gn (go t)
-      | GenNode 10 [FLOAT_TYPE sz] => Tfloat_ sz
-      | GenNode 11 [QUAL q; t] => Tqualified q (go t)
-      | GenNode 12 [] => Tnullptr
-      | GenNode 13 [BS gn] => Tarch None gn
-      | GenNode 14 [BITSIZE sz; BS gn] => Tarch (Some sz) gn
-      | GenNode 15 [BS gn] => Tenum gn
-      | GenNode 16 [CHAR_TYPE sz] => Tchar_ sz
-      | GenNode 19 [BS msg] => Tunsupported msg
-      | _ => Tvoid	(** dummy *)
-      end.
-    apply (inj_countable' enc dec). refine (fix go t := _).
-    destruct t as [| | | | | | | | | | |cc ar ret args| | | | | |[]|]; simpl; f_equal; try done.
-    induction args; simpl; f_equal; done.
-  Defined.
-End type_countable.
-
-(**
-An equivalence relation on types that quotients by "identical to C++".
-The equations here are dictated by the fact that [type] is too big for
-C++.
-*)
-
-Inductive type_equiv : Equiv type :=
-
-(**
-Qualifier normalization
-*)
-| Tqualified_id t : Tqualified QM t ≡ t
-| Tqualified_merge q q' t : Tqualified q (Tqualified q' t) ≡ Tqualified (merge_tq q q') t
-(*
-"An array type whose elements are cv-qualified is also considered to
-have the same cv-qualifications as its elements. [...] Cv-qualifiers
-applied to an array type attach to the underlying element type."
-<https://www.eel.is/c++draft/basic.type.qualifier#3>
-*)
-| Tqualified_array q t n : Tqualified q (Tarray t n) ≡ Tarray (Tqualified q t) n
-(*
-"A function or reference type is always cv-unqualified."
-<https://www.eel.is/c++draft/basic.type.qualifier#1>
-*)
-| Tqualified_ref q t : Tqualified q (Tref t) ≡ Tref t
-| Tqualified_rv_ref q t : Tqualified q (Trv_ref t) ≡ Trv_ref t
-| Tqualified_func q cc ar ret args : Tqualified q (@Tfunction cc ar ret args) ≡ @Tfunction cc ar ret args
-(**
-"After producing the list of parameter types, any top-level
-cv-qualifiers modifying a parameter type are deleted when forming the
-function type."
-<https://www.eel.is/c++draft/dcl.fct#5>
-*)
-| Tqualified_func_param cc ar ret q t args args' : @Tfunction cc ar ret (args ++ Tqualified q t :: args') ≡ @Tfunction cc ar ret (args ++ t :: args')
-
-(** Equivalence *)
-| type_equiv_refl t : t ≡ t
-| type_equiv_sym t u : t ≡ u -> u ≡ t
-| type_equiv_trans t u v : t ≡ u -> u ≡ v -> t ≡ v
-
-(** Compatibility *)
-| Tptr_proper : Proper (equiv ==> equiv) Tptr
-| Tref_proper : Proper (equiv ==> equiv) Tref
-| Trv_ref_proper : Proper (equiv ==> equiv) Trv_ref
-| Tarray_proper : Proper (equiv ==> eq ==> equiv) Tarray
-| Tfunction_proper cc ar : Proper (equiv ==> equiv ==> equiv) (@Tfunction cc ar)
-| Tmember_pointer_proper gn : Proper (equiv ==> equiv) (Tmember_pointer gn)
-| Tqualified_proper q : Proper (equiv ==> equiv) (Tqualified q)
-.
-#[global] Existing Instances
-  type_equiv
-  Tptr_proper
-  Tref_proper
-  Trv_ref_proper
-  Tarray_proper
-  Tfunction_proper
-  Tmember_pointer_proper
-  Tqualified_proper
-.
-#[global] Instance type_equivalence : Equivalence (≡@{type}) :=
-  Build_Equivalence _ type_equiv_refl type_equiv_sym type_equiv_trans.
-
-Notation Tpointer := Tptr (only parsing).
-Notation Treference := Tref (only parsing).
-Notation Trv_reference := Trv_ref (only parsing).
-Notation Tfun := Tfunction (only parsing).
-
-Definition Qconst_volatile : type -> type :=
-  Tqualified QCV.
-Definition Qconst : type -> type :=
-  Tqualified QC.
-Definition Qvolatile : type -> type :=
-  Tqualified QV.
-Notation Qmut_volatile := Qvolatile (only parsing).
-Definition Qmut : type -> type :=
-  Tqualified QM.
-
-#[global] Hint Opaque
-  Qconst_volatile Qconst Qvolatile Qmut
-: typeclass_instances.
-
-#[global] Instance Qconst_volatile_proper : Proper (equiv ==> equiv) Qconst_volatile.
-Proof. solve_proper. Qed.
-#[global] Instance Qconst_proper : Proper (equiv ==> equiv) Qconst.
-Proof. solve_proper. Qed.
-#[global] Instance Qvolatile_proper : Proper (equiv ==> equiv) Qvolatile.
-Proof. solve_proper. Qed.
-#[global] Instance Qmut_proper : Proper (equiv ==> equiv) Qmut.
-Proof. solve_proper. Qed.
-
-Lemma Qmut_equiv t : Qmut t ≡ t.
-Proof. by rewrite /Qmut Tqualified_id. Qed.
+Section with_lang.
+  Context {lang : lang.t}.
+  #[local] Notation type := (type' lang).
 
 (** ** Qualifier normalization *)
 (**
@@ -566,8 +22,7 @@ returns them, paired with the rest of the type.
 
 The underlying functions [qual_norm] and [qual_norm'] are similar
 (see, e.g., [qual_norm_decompose_type]).
-*)
-
+ *)
 Section qual_norm.
   Context {A : Type}.
   Variable f : type_qualifiers -> type -> A.
@@ -603,14 +58,136 @@ Definition decompose_type : type -> type_qualifiers * type :=
 #[global] Arguments decompose_type !_ / : simpl nomatch, assert.
 
 (**
-[drop_qualifiers t] drops all the *leading* qualifiers of the type [t],
-e.g. [drop_qualifiers (Qconst (Qmut t)) = t].
- *)
+[take_qualifiers], [drop_qualifiers] return and remove leading
+qualifiers.
+*)
+Definition take_qualifiers : type -> type_qualifiers :=
+  qual_norm (fun cv _ => cv).
+
 Fixpoint drop_qualifiers (t : type) : type :=
   match t with
   | Tqualified _ t => drop_qualifiers t
   | _ => t
   end.
+
+(**
+[drop_reference] removes any leading reference types.
+*)
+Fixpoint drop_reference (t : type) : exprtype' lang :=
+  match drop_qualifiers t with
+  | Tref u | Trv_ref u => drop_reference u
+  | _ => t	(* We do not normalize qualifiers here to promote sharing *)
+  end.
+
+Succeed Example TEST_drop_reference : drop_reference (Qconst Tint) = Qconst Tint := eq_refl.
+Succeed Example TEST_drop_reference : drop_reference (Qconst (Tref Tint)) = Tint := eq_refl.
+Succeed Example TEST_drop_reference : drop_reference (Qconst (Tref (Qconst Tint))) = Qconst Tint := eq_refl.
+
+(** ** Smart constructors *)
+
+(**
+Qualify a type, merging nested qualifiers, suppressing [QM]
+qualifiers, and (https://www.eel.is/c++draft/dcl.ref#1) discarding any
+cv-qualifiers on reference types.
+*)
+Definition tqualified' (q : type_qualifiers) (t : type) : type :=
+  match t with
+  | Tref _ | Trv_ref _ => t
+  | _ => match q with QM => t | _ => Tqualified q t end
+  end.
+#[global] Hint Opaque tqualified' : typeclass_instances.
+#[global] Arguments tqualified' _ !_ / : simpl nomatch, assert.
+
+Definition tqualified : type_qualifiers -> type -> type :=
+  qual_norm' tqualified'.
+#[global] Hint Opaque tqualified : typeclass_instances.
+#[global] Arguments tqualified _ !_ / : simpl nomatch, assert.
+
+(**
+[tref], [trv_ref] implement reference collapsing.
+
+Background:
+https://en.cppreference.com/w/cpp/language/reference#Reference_collapsing
+https://www.eel.is/c++draft/dcl.ref#6
+https://www.eel.is/c++draft/dcl.ref#5
+*)
+Definition tref := fix tref (acc : type_qualifiers) (t : type) : type :=
+  match t with
+  | Tref t | Trv_ref t => tref QM t
+  | Tqualified q t => tref (merge_tq acc q) t
+  | _ => Tref (tqualified acc t)
+  end.
+#[global] Hint Opaque tref : typeclass_instances.
+#[global] Arguments tref _ !_ / : simpl nomatch, assert.
+
+Definition trv_ref := fix trv_ref (acc : type_qualifiers) (t : type) : type :=
+  match t with
+  | Tref t => tref QM t
+  | Trv_ref t => trv_ref QM t
+  | Tqualified q t => trv_ref (merge_tq acc q) t
+  | _ => Trv_ref (tqualified acc t)
+  end.
+#[global] Hint Opaque trv_ref : typeclass_instances.
+#[global] Arguments trv_ref _ !_ / : simpl nomatch, assert.
+
+(**
+An equivalence relation on types that quotients by "identical to C++".
+The equations here are dictated by the fact that [type] is too big for
+C++.
+*)
+
+Inductive type_equiv : Equiv type :=
+(** Equivalence *)
+| type_equiv_refl t : t ≡ t
+| type_equiv_sym t u : t ≡ u -> u ≡ t
+| type_equiv_trans t u v : t ≡ u -> u ≡ v -> t ≡ v
+
+(** Compatibility *)
+| Tptr_proper : Proper (equiv ==> equiv) Tptr
+| Tref_proper : Proper (equiv ==> equiv) Tref
+| Trv_ref_proper : Proper (equiv ==> equiv) Trv_ref
+| Tarray_proper : Proper (equiv ==> eq ==> equiv) Tarray
+(* | Tfunction_proper cc ar : Proper (equiv ==> equiv ==> equiv) (@Tfunction lang cc ar) *)
+| Tmember_pointer_proper gn : Proper (equiv ==> equiv) (Tmember_pointer gn)
+| Tqualified_proper q : Proper (equiv ==> equiv) (Tqualified q)
+.
+#[global] Existing Instances
+  type_equiv
+  Tptr_proper
+  Tref_proper
+  Trv_ref_proper
+  Tarray_proper
+  Tmember_pointer_proper
+  Tqualified_proper
+.
+#[global] Instance type_equivalence : Equivalence (≡@{type}) :=
+  Build_Equivalence _ type_equiv_refl type_equiv_sym type_equiv_trans.
+
+Definition Qconst_volatile : type -> type :=
+  Tqualified QCV.
+Definition Qconst : type -> type :=
+  Tqualified QC.
+Definition Qvolatile : type -> type :=
+  Tqualified QV.
+Notation Qmut_volatile := Qvolatile (only parsing).
+Definition Qmut : type -> type :=
+  Tqualified QM.
+
+#[global] Hint Opaque
+  Qconst_volatile Qconst Qvolatile Qmut
+: typeclass_instances.
+
+#[global] Instance Qconst_volatile_proper : Proper (equiv ==> equiv) Qconst_volatile.
+Proof. solve_proper. Qed.
+#[global] Instance Qconst_proper : Proper (equiv ==> equiv) Qconst.
+Proof. solve_proper. Qed.
+#[global] Instance Qvolatile_proper : Proper (equiv ==> equiv) Qvolatile.
+Proof. solve_proper. Qed.
+#[global] Instance Qmut_proper : Proper (equiv ==> equiv) Qmut.
+Proof. solve_proper. Qed.
+
+Lemma Qmut_equiv t : Qmut t ≡ t.
+Proof. (* by rewrite /Qmut Tqualified_id. *) Admitted. (* type_equiv *)
 
 (**
 It would be nice to make this the default.
@@ -665,7 +242,7 @@ Section qual_norm.
 
   Lemma qual_norm'_ok f q t : qual_norm_spec f q t (qual_norm' f q t).
   Proof.
-    move: q. induction t=>q.
+    move: q. induction t; intros.
     all: rewrite qual_norm'_unfold; auto.
   Qed.
 
@@ -718,10 +295,10 @@ Lemma qual_norm'_equiv q t : qual_norm' Tqualified q t ≡ Tqualified q t.
 Proof.
   induction (qual_norm'_ok Tqualified q t).
   { done. }
-  { by rewrite Tqualified_merge. }
-Qed.
+  { (* by rewrite Tqualified_merge. }
+Qed. *) Admitted. (* type_equiv *)
 Lemma qual_norm_equiv t : qual_norm Tqualified t ≡ t.
-Proof. by rewrite /qual_norm qual_norm'_equiv Tqualified_id. Qed.
+Proof. (* by rewrite /qual_norm qual_norm'_equiv Tqualified_id. Qed. *) Admitted. (* type_equiv *)
 
 (** [decompose_type] *)
 
@@ -731,12 +308,12 @@ Lemma decompose_type_unfold t :
       let p := decompose_type t' in
       (merge_tq q p.1, p.2)
     else (QM, t).
-Proof.
+Proof. (*
   rewrite /decompose_type qual_norm_unfold.
   destruct t as [| | | | | | | | | | | | | | |q t| | |]; try done. set pair := fun x y => (x, y).
   move: q. induction t=>q; cbn; try by rewrite right_id_L.
   rewrite left_id_L !IHt /=. f_equal. by rewrite assoc_L.
-Qed.
+Qed. *) Admitted. (* TODO *)
 
 Inductive decompose_type_spec : type -> type_qualifiers * type -> Prop :=
 | decompose_type_spec_unqual t : ~~ is_qualified t -> decompose_type_spec t (QM, t)
@@ -754,7 +331,6 @@ Qed.
 
 Lemma is_qualified_decompose_type t : ~~ is_qualified (decompose_type t).2.
 Proof. by induction (decompose_type_ok t). Qed.
-#[global] Hint Resolve is_qualified_decompose_type | 0 : core.
 
 Lemma decompose_type_unqual t : ~~ is_qualified t -> decompose_type t = (QM, t).
 Proof. apply qual_norm_unqual. Qed.
@@ -767,14 +343,14 @@ Proof. by rewrite decompose_type_unfold. Qed.
 
 Lemma decompose_type_idemp t :
   decompose_type (decompose_type t).2 = (QM, (decompose_type t).2).
-Proof. by rewrite decompose_type_unqual. Qed.
+Proof. (* by rewrite decompose_type_unqual. Qed. *) Admitted. (* type_equiv *)
 
 Lemma decompose_type_equiv t : let p := decompose_type t in Tqualified p.1 p.2 ≡ t.
-Proof.
+Proof. (*
   elim: (decompose_type_ok t); cbn.
   { intros. by rewrite Tqualified_id. }
   { intros ???? <-. by rewrite Tqualified_merge. }
-Qed.
+Qed. *) Admitted. (* type_equiv *)
 
 (** [qual_norm], [qual_norm'] in terms of [decompose_type] *)
 
@@ -782,10 +358,10 @@ Lemma qual_norm'_decompose_type {A} (f : type_qualifiers -> type -> A) q t :
   qual_norm' f q t =
     let p := decompose_type t in
     f (merge_tq q p.1) p.2.
-Proof.
+Proof. (*
   move: q. induction t=>q /=; try by rewrite right_id_L.
   rewrite decompose_type_unfold IHt /=. by rewrite assoc_L.
-Qed.
+Qed. *) Admitted. (* FIXME *)
 
 Lemma qual_norm_decompose_type {A} (f : type_qualifiers -> type -> A) t :
   qual_norm f t =
@@ -800,7 +376,7 @@ Qed.
 
 Lemma is_qualified_drop_qualifiers ty : ~~ is_qualified (drop_qualifiers ty).
 Proof. by induction ty. Qed.
-#[global] Hint Resolve is_qualified_drop_qualifiers | 0 : core.
+#[local] Hint Resolve is_qualified_drop_qualifiers | 0 : core. (* TODO: make this global? *)
 
 Lemma drop_qualifiers_unqual t : ~~ is_qualified t -> drop_qualifiers t = t.
 Proof. by destruct t; cbn; auto. Qed.
@@ -844,7 +420,7 @@ the other criteria.
 *)
 Fixpoint erase_qualifiers (t : type) : type :=
   match t with
-  | Tpointer t => Tpointer (erase_qualifiers t)
+  | Tptr t => Tptr (erase_qualifiers t)
   | Tref t => Tref (erase_qualifiers t)
   | Trv_ref t => Trv_ref (erase_qualifiers t)
   | Tnum _ _
@@ -856,18 +432,25 @@ Fixpoint erase_qualifiers (t : type) : type :=
   | Tenum _ => t
   | Tarray t sz => Tarray (erase_qualifiers t) sz
   | Tincomplete_array t => Tincomplete_array (erase_qualifiers t)
-  | Tvariable_array t => Tvariable_array (erase_qualifiers t)
-  | @Tfunction cc ar t ts => Tfunction (cc:=cc) (ar:=ar) (erase_qualifiers t) (List.map erase_qualifiers ts)
+  | Tvariable_array t e => Tvariable_array (erase_qualifiers t) e
+  | Tfunction ft => Tfunction $ FunctionType (ft_cc:=ft.(ft_cc)) (ft_arity:=ft.(ft_arity)) (erase_qualifiers ft.(ft_return)) (List.map erase_qualifiers ft.(ft_params))
   | Tmember_pointer cls t => Tmember_pointer cls (erase_qualifiers t)
   | Tqualified _ t => erase_qualifiers t
   | Tnullptr => Tnullptr
   | Tarch sz nm => Tarch sz nm
   | Tunsupported msg => Tunsupported msg
+  | Tparam _
+  | Tresult_param _
+  | Tresult_global _
+  | Tresult_unop _ _ | Tresult_binop _ _ _ | Tresult_call _ _ | Tresult_member_call _ _ _
+  | Tresult_parenlist _ _
+  | Tresult_member _ _
+  | Tdecltype _ => t (* TODO: it isn't clear what [erase_qualifiers] means on meta types *)
   end.
 
 Lemma is_qualified_erase_qualifiers ty : ~~ is_qualified (erase_qualifiers ty).
 Proof. by induction ty. Qed.
-#[global] Hint Resolve is_qualified_erase_qualifiers | 0 : core.
+#[local] Hint Resolve is_qualified_erase_qualifiers | 0 : core. (* TODO: global *)
 
 Lemma erase_qualifiers_qual_norm' q t :
   erase_qualifiers t = qual_norm' (fun _ t => erase_qualifiers t) q t.
@@ -882,8 +465,8 @@ Proof. by rewrite erase_qualifiers_qual_norm qual_norm_decompose_type. Qed.
 Lemma erase_qualifiers_idemp t : erase_qualifiers (erase_qualifiers t) = erase_qualifiers t.
 Proof.
   move: t. fix IHt 1=>t.
-  destruct t as [| | | | | | | | | | |cc ar ret args| | | | | | |]; cbn; auto with f_equal.
-  { (* functions *) rewrite IHt. f_equal. induction args; cbn; auto with f_equal. }
+  destruct t (*as [| | | | | | | | | | |cc ar ret args| | | | | | |] *); cbn; auto with f_equal.
+  { (* functions *) rewrite IHt. f_equal. f_equal. induction (ft_params t); cbn; auto with f_equal. }
 Qed.
 
 Lemma drop_erase_qualifiers t : drop_qualifiers (erase_qualifiers t) = erase_qualifiers t.
@@ -928,10 +511,12 @@ Proof. induction ty; simpl; intros; try congruence; eauto. Qed.
 Lemma drop_qualifiers_Tenum : forall [ty nm],
     drop_qualifiers ty = Tenum nm -> erase_qualifiers ty = Tenum nm.
 Proof. induction ty; simpl; intros; try congruence; eauto. Qed.
+(* TODO function types
 Lemma drop_qualifiers_Tfunction : forall [ty c ar ty' tArgs],
     drop_qualifiers ty = @Tfunction c ar ty' tArgs ->
     erase_qualifiers ty = @Tfunction c ar (erase_qualifiers ty') (map erase_qualifiers tArgs).
 Proof. induction ty; simpl; intros; try congruence; eauto. Qed.
+*)
 Lemma drop_qualifiers_Tbool : forall [ty],
     drop_qualifiers ty = Tbool -> erase_qualifiers ty = Tbool.
 Proof. induction ty; simpl; intros; try congruence; eauto. Qed.
@@ -961,72 +546,13 @@ Ltac simpl_drop_qualifiers :=
           | rewrite (drop_qualifiers_Tarray H)
           | rewrite (drop_qualifiers_Tnamed H)
           | rewrite (drop_qualifiers_Tenum H)
-          | rewrite (drop_qualifiers_Tfunction H)
+(*          | rewrite (drop_qualifiers_Tfunction H) *)
           | rewrite (drop_qualifiers_Tbool H)
           | rewrite (drop_qualifiers_Tmember_pointer H)
           | rewrite (drop_qualifiers_Tfloat H)
           | rewrite (drop_qualifiers_Tnullptr H)
           ]
   end.
-
-(** ** Smart constructors *)
-
-(**
-Qualify a type, merging nested qualifiers, suppressing [QM]
-qualifiers, and (https://www.eel.is/c++draft/dcl.ref#1) discarding any
-cv-qualifiers on reference types.
-*)
-Definition tqualified' (q : type_qualifiers) (t : type) : type :=
-  match t with
-  | Tref _ | Trv_ref _ => t
-  | _ => match q with QM => t | _ => Tqualified q t end
-  end.
-#[global] Hint Opaque tqualified' : typeclass_instances.
-#[global] Arguments tqualified' _ !_ / : simpl nomatch, assert.
-
-Definition tqualified : type_qualifiers -> type -> type :=
-  qual_norm' tqualified'.
-#[global] Hint Opaque tqualified : typeclass_instances.
-#[global] Arguments tqualified _ !_ / : simpl nomatch, assert.
-
-(**
-[drop_reference t] removes any leading reference types.
-*)
-Fixpoint drop_reference (t : type) : exprtype :=
-  match drop_qualifiers t with
-  | Tref u | Trv_ref u => drop_reference u
-  | _ => t	(** We do not normalize qualifiers here to promote sharing *)
-  end.
-
-Succeed Example TEST_drop_reference : drop_reference (Qconst (Tnamed "T")) = Qconst (Tnamed "T") := eq_refl.
-Succeed Example TEST_drop_reference : drop_reference (Qconst (Tref (Tnamed "T"))) = Tnamed "T" := eq_refl.
-Succeed Example TEST_drop_reference : drop_reference (Qconst (Tref (Qconst $ Tnamed "T"))) = Qconst (Tnamed "T") := eq_refl.
-
-(**
-[tref], [trv_ref] implement reference collapsing.
-
-Background:
-https://en.cppreference.com/w/cpp/language/reference#Reference_collapsing
-https://www.eel.is/c++draft/dcl.ref#5
-*)
-Fixpoint tref (acc : type_qualifiers) (t : type) : type :=
-  match t with
-  | Tref t | Trv_ref t => tref QM t
-  | Tqualified q t => tref (merge_tq acc q) t
-  | _ => Tref (tqualified acc t)
-  end.
-#[global] Hint Opaque tref : typeclass_instances.
-#[global] Arguments tref _ !_ / : simpl nomatch, assert.
-
-Fixpoint trv_ref (acc : type_qualifiers) (t : type) : type :=
-  match t with
-  | Tref t => tref QM t
-  | Trv_ref t => trv_ref QM t
-  | Tqualified q t => trv_ref (merge_tq acc q) t
-  | _ => Trv_ref (tqualified acc t)
-  end.
-#[global] Hint Opaque trv_ref : typeclass_instances.
-#[global] Arguments trv_ref _ !_ / : simpl nomatch, assert.
 
 (**
 [is_ref t] decides if [t] a reference type
@@ -1074,13 +600,13 @@ Proof.
 Qed.
 
 Lemma tqualified'_equiv q t : tqualified' q t ≡ Tqualified q t.
-Proof.
+Proof. (*
   case: (tqualified'_ok q t).
   { intros ?? (?&[-> | ->])%is_ref_spec.
     by rewrite Tqualified_ref. by rewrite Tqualified_rv_ref. }
   { intros. by rewrite Tqualified_id. }
   { done. }
-Qed.
+Qed. *) Admitted. (* type_equiv *)
 
 #[global] Instance: Params (@tqualified') 1 := {}.
 #[global] Instance tqualified'_proper q : Proper (equiv ==> equiv) (tqualified' q).
@@ -1102,8 +628,8 @@ Lemma tqualified_equiv q t : tqualified q t ≡ Tqualified q t.
 Proof.
   induction (tqualified_ok q t).
   { by rewrite tqualified'_equiv. }
-  { by rewrite Tqualified_merge. }
-Qed.
+  { (* by rewrite Tqualified_merge. }
+Qed. *) Admitted. (* type_equiv *)
 
 #[global] Instance: Params (@tqualified) 1 := {}.
 #[global] Instance tqualified_proper q : Proper (equiv ==> equiv) (tqualified q).
@@ -1164,7 +690,7 @@ Inductive tref_spec : type_qualifiers -> type -> type -> Prop :=
 #[local] Hint Constructors tref_spec : core.
 
 Lemma tref_ok q t : tref_spec q t (tref q t).
-Proof. move: q. induction t=>q; auto. Qed.
+Proof. revert q. induction t; auto. Qed.
 
 (*
 Lemma tref_equiv' q t : tref q t ≡ Tref (Tqualified q t).
@@ -1204,7 +730,7 @@ Inductive trv_ref_spec : type_qualifiers -> type -> type -> Prop :=
 #[local] Hint Constructors trv_ref_spec : core.
 
 Lemma trv_ref_ok q t : trv_ref_spec q t (trv_ref q t).
-Proof. move: q; induction t=>q; auto. Qed.
+Proof. revert q; induction t; auto. Qed.
 
 (*
 Lemma trv_ref_equiv' q t : trv_ref q t ≡ Trv_ref (Tqualified q t).
@@ -1247,14 +773,14 @@ Fixpoint normalize_type (t : type) : type :=
     qual_norm' (fun q t => tqualified q (normalize_type t))
   in
   match t with
-  | Tpointer t => Tpointer (normalize_type t)
+  | Tptr t => Tptr (normalize_type t)
   | Tref t => Tref (normalize_type t)
   | Trv_ref t => Trv_ref (normalize_type t)
   | Tarray t n => Tarray (normalize_type t) n
   | Tincomplete_array t => Tincomplete_array (normalize_type t)
-  | Tvariable_array t => Tvariable_array (normalize_type t)
-  | @Tfunction cc ar r args =>
-    Tfunction (cc:=cc) (ar:=ar) (normalize_type r) (List.map drop_norm args)
+  | Tvariable_array t e => Tvariable_array (normalize_type t) e
+  | Tfunction ft (* cc ar r args *) =>
+    Tfunction $ FunctionType (ft_cc:=ft.(ft_cc)) (ft_arity:=ft.(ft_arity)) (normalize_type ft.(ft_return)) (List.map drop_norm ft.(ft_params))
   | Tmember_pointer gn t => Tmember_pointer gn (normalize_type t)
   | Tqualified q t => qual_norm q t
   | Tnum _ _ => t
@@ -1267,8 +793,16 @@ Fixpoint normalize_type (t : type) : type :=
   | Tfloat_ _ => t
   | Tarch _ _ => t
   | Tunsupported _ => t
+  | Tparam _
+  | Tresult_param _
+  | Tresult_global _
+  | Tresult_unop _ _ | Tresult_binop _ _ _ | Tresult_call _ _ | Tresult_member_call _ _ _
+  | Tresult_parenlist _ _
+  | Tresult_member _ _
+  | Tdecltype _ => t (* TODO: it isn't clear what [normalize_type] means on meta types *)
   end.
 
+(*
 Section normalize_type_idempotent.
 
   Fixpoint _drop_norm_idempotent q q' ty {struct ty}:
@@ -1316,6 +850,7 @@ End normalize_type_idempotent.
 Lemma normalize_type_qual_norm t :
   normalize_type t = qual_norm (fun q t' => tqualified q (normalize_type t')) t.
 Proof. rewrite qual_norm_unfold. by destruct t. Qed.
+*)
 
 (** ** Qualifier-aware type operations *)
 
@@ -1332,7 +867,7 @@ Definition unptr (t : type) : option type :=
 (**
 [class_name t] returns the name of the class that this type refers to
 *)
-Definition class_name (t : type) : option globname :=
+Definition class_name (t : type) : option (name' lang) :=
   match drop_qualifiers t with
   | Tnamed gn => Some gn
   | _ => None
@@ -1444,7 +979,7 @@ Proof.
   induction t; simpl; intros; auto.
   { rewrite qual_norm_unfold. rewrite /qual_norm/=.
     rewrite -IHt. rewrite {2}/zero_sized_array.
-    destruct t0; auto. }
+    destruct q0; auto. }
 Qed.
 Lemma zero_sized_array_erase_qualifiers t :
   zero_sized_array t = zero_sized_array (erase_qualifiers t).
@@ -1503,12 +1038,12 @@ return the underlying type [u] (defaulting, respectively, to a dummy
 type and to [None]).
 *)
 
-Definition as_ref' {A} (f : exprtype -> A) (x : A) (t : type) : A :=
+Definition as_ref' {A} (f : exprtype' lang -> A) (x : A) (t : type) : A :=
   if drop_qualifiers t is (Tref u | Trv_ref u) then f u else x.
 Notation as_ref := (as_ref' (fun u => u) Tvoid).
 Notation as_ref_option := (as_ref' Some None).
 
-Lemma as_ref'_erase_qualifiers {A} (f : exprtype -> A) (x : A) t :
+Lemma as_ref'_erase_qualifiers {A} (f : exprtype' lang -> A) (x : A) t :
   as_ref' f x (erase_qualifiers t) = as_ref' (f ∘ erase_qualifiers) x t.
 Proof. induction t; cbn; auto. Qed.
 Lemma as_ref_erase_qualifiers t :
@@ -1516,7 +1051,7 @@ Lemma as_ref_erase_qualifiers t :
 Proof. induction t; cbn; auto. Qed.
 
 Section as_ref'.
-  Context {A : Type} (f : exprtype -> A) (x : A).
+  Context {A : Type} (f : exprtype' lang -> A) (x : A).
   #[local] Notation as_ref' := (as_ref' f x).
 
   Lemma as_ref_drop_qualifiers t : as_ref' (drop_qualifiers t) = as_ref' t.
@@ -1618,70 +1153,22 @@ Qed.
 Definition is_volatile : type -> bool :=
   qual_norm (fun cv _ => q_volatile cv).
 
-(** ** Notation for character types *)
-Coercion Tchar_ : char_type.t >-> type.
-Notation Tchar   := (Tchar_ char_type.Cchar).
-Notation Twchar  := (Tchar_ char_type.Cwchar).
-Notation Tchar8  := (Tchar_ char_type.C8).
-Notation Tchar16 := (Tchar_ char_type.C16).
-Notation Tchar32 := (Tchar_ char_type.C32).
+(* [Tmember_func ty fty] constructs the function type for a
+     member function that takes a [this] parameter of [ty]
 
-(** ** Types with explicit size information. *)
-
-Notation Ti8    := (Tnum W8 Signed).
-Notation Tu8    := (Tnum W8 Unsigned).
-Notation Ti16   := (Tnum W16 Signed).
-Notation Tu16   := (Tnum W16 Unsigned).
-Notation Ti32   := (Tnum W32 Signed).
-Notation Tu32   := (Tnum W32 Unsigned).
-Notation Ti64   := (Tnum W64 Signed).
-Notation Tu64   := (Tnum W64 Unsigned).
-Notation Ti128  := (Tnum W128 Signed).
-Notation Tu128  := (Tnum W128 Unsigned).
-
-(* note(gmm): types without explicit size information need to
- * be parameters of the underlying code, otherwise we can't
- * describe the semantics correctly.
- * - cpp2v should probably insert these types.
+   TODO technically the [this] parameter is [const].
  *)
-(**
-<https://en.cppreference.com/w/cpp/language/types>
-The 4 definitions below use the LP64 data model.
-LLP64 and LP64 agree except for the [long] type: see
-the warning below.
-In future, we may want to parametrize by a data model, or
-the machine word size.
-(** warning: LLP64 model uses [long_bits := W32] *)
-*)
-Notation char_bits      := (int_type.Ichar)     (only parsing).
-Notation short_bits     := (int_type.Ishort)    (only parsing).
-Notation int_bits       := (int_type.Iint)      (only parsing).
-Notation long_bits      := (int_type.Ilong)     (only parsing).
-Notation long_long_bits := (int_type.Ilonglong) (only parsing).
+Definition Tmember_func {lang} (ty : exprtype' lang) (fty : functype' lang) : functype' lang :=
+  match fty with
+  | Tfunction ft => Tfunction $ {| ft_cc := ft.(ft_cc) ; ft_arity := ft.(ft_arity)
+                                ; ft_return := ft.(ft_return) ; ft_params := Tptr ty :: ft.(ft_params) |}
+  | _ => fty
+  end.
 
-(* TODO: this is correct in the LP64 data model, but we will probably need to
- * index this by the [genv] in the future. *)
-Notation Tsize_t := Tu64 (only parsing).
 
-(** ** Types with implicit size information. *)
+End with_lang.
 
-Notation Tschar  := (Tnum int_type.Ichar Signed) (only parsing).
-Notation Tuchar  := (Tnum int_type.Ichar Unsigned) (only parsing).
-
-Notation Tushort := (Tnum int_type.Ishort Unsigned) (only parsing).
-Notation Tshort  := (Tnum int_type.Ishort Signed) (only parsing).
-
-Notation Tint  := (Tnum int_type.Iint Signed) (only parsing).
-Notation Tuint := (Tnum int_type.Iint Unsigned) (only parsing).
-
-Notation Tulong := (Tnum int_type.Ilong Unsigned) (only parsing).
-Notation Tlong  := (Tnum int_type.Ilong Signed) (only parsing).
-
-Notation Tulonglong := (Tnum int_type.Ilonglong Unsigned) (only parsing).
-Notation Tlonglong  := (Tnum int_type.Ilonglong Signed) (only parsing).
-
-Notation Tfloat16 := (Tfloat_ float_type.Ffloat16).
-Notation Tfloat := (Tfloat_ float_type.Ffloat).
-Notation Tdouble := (Tfloat_ float_type.Fdouble).
-Notation Tlongdouble := (Tfloat_ float_type.Flongdouble).
-Notation Tfloat128 := (Tfloat_ float_type.Ffloat128).
+Notation as_ref := (as_ref' (fun u => u) Tvoid).
+Notation as_ref_option := (as_ref' Some None).
+#[global] Hint Resolve is_qualified_decompose_type | 0 : core.
+#[global] Hint Resolve is_qualified_drop_qualifiers | 0 : core.
