theories/lang/cpp/logic/stmt.v
@@ -8,7 +8,7 @@ Require Import bedrock.lang.proofmode.proofmode.
 Require Import bedrock.lang.bi.atomic_commit.
 Require Import bedrock.lang.bi.spec.exclusive.
 
-Require Import bedrock.lang.cpp.ast.
+Require Import bedrock.lang.cpp.syntax.
 Require Import bedrock.lang.cpp.semantics.
 Require Import bedrock.lang.cpp.logic.pred.
 Require Import bedrock.lang.cpp.logic.path_pred.
