theories/lang/cpp/logic/wp_notations.v
@@ -3,7 +3,7 @@
  * This software is distributed under the terms of the BedRock Open-Source License.
  * See the LICENSE-BedRock file in the repository root for details.
  *)
-Require Import bedrock.lang.cpp.syntax.names.
+Require Import bedrock.lang.cpp.syntax.
 Require Import bedrock.lang.cpp.logic.
 Require Import bedrock.lang.cpp.logic.atomics.
 Require Import bedrock.lang.cpp.logic.builtins.
