theories/lang/cpp/parser/stmt.v
@@ -1,0 +1,46 @@
+(*
+ * Copyright (c) 2024 BedRock Systems, Inc.
+ * This software is distributed under the terms of the BedRock Open-Source License.
+ * See the LICENSE-BedRock file in the repository root for details.
+ *)
+Require Import bedrock.prelude.bytestring.
+Require Import bedrock.lang.cpp.parser.prelude.
+
+#[local] Open Scope bs_scope.
+
+(* TODO: remove these next definitiosn when we drop [DTOR] *)
+Fixpoint do_end (ty : bs) : bs :=
+  match ty with
+  | BS.String _ BS.EmptyString => "D0Ev"
+  | BS.String x v => BS.String x (do_end v)
+  | _ => BS.EmptyString
+  end.
+
+(** Build the name of a destructor for a type.
+    NOTE this can be improved if we essentially turn it into a
+    constructor of [obj_name]; however, that has some wider
+    implications that we should solve in a separate issue.
+ *)
+Definition DTOR (ty : bs) : bs :=
+  match ty with
+  | BS.String _ (BS.String _ ((BS.String c _) as rest)) =>
+      if bool_decide (c = "N"%byte) then
+        "_Z" ++ do_end rest
+      else
+        "_ZN" ++ rest ++ "D0Ev"
+  | BS.String _ (BS.String _ v) => "_ZN" ++ do_end v
+  | _ => "OOPS"
+  end%bs.
+
+Section stmt.
+  Context {lang : lang.t}.
+  #[local] Notation Expr := (Expr' lang).
+  #[local] Notation Stmt := (Stmt' lang).
+
+  Definition Sreturn_void : Stmt := Sreturn None.
+  Definition Sreturn_val (e : Expr) : Stmt := Sreturn (Some e).
+  Definition Sforeach (range ibegin iend : Stmt)
+    (init : option Stmt) (cond : option Expr) (inc : option Expr)
+    (decl body : Stmt) : Stmt :=
+    Sseq [range; ibegin; iend; Sfor init cond inc (Sseq [decl; body])].
+End stmt.
