theories/lang/cpp/syntax/notations.v
@@ -1,0 +1,32 @@
+(*
+ * Copyright (c) 2024 BedRock Systems, Inc.
+ * This software is distributed under the terms of the BedRock Open-Source License.
+ * See the LICENSE-BedRock file in the repository root for details.
+ *)
+Require Import bedrock.lang.cpp.parser.notation.
+
+Declare Scope cpp_scope.
+Delimit Scope cpp_scope with cpp.
+
+Declare Scope cppfield_scope.
+Delimit Scope cppfield_scope with field.
+
+Declare Scope cppname_scope.
+Delimit Scope cppname_scope with cppname.
+
+(* XXX This is only parsing to work around Coq misusing it outside
+[cppfield_scope]. See #235. *)
+Notation "` e `" := e (e custom cppglobal at level 200, at level 0,
+                        only parsing) : cppfield_scope.
+Notation "` e `" := e (e custom cppglobal at level 200, at level 0,
+                        only parsing) : cppname_scope.
+
+
+(** Importing [cpp_notation] makes cpp2v-generated names generally
+available as, e.g., [``::MyClass``]. *)
+Module Export cpp_notation.
+  Notation "'``' e '``'" := e
+                              (at level 0, e custom cppglobal at level 200,
+                                format "`` e ``") : cpp_scope.
+  Open Scope cpp_scope.
+End cpp_notation.
