theories/lang/cpp/syntax/templates.v
@@ -1,0 +1,61 @@
+Require Import bedrock.prelude.base.
+Require Import bedrock.lang.cpp.syntax.core.
+
+(** ** Template pre-instances *)
+(**
+A template file maps the symbol or type name of a template
+instantiation (bound in a translation unit) to a _template
+pre-instance_ comprising the instance's template name (bound in a
+template file) and arguments.
+*)
+Definition temp_name : Set := name' lang.temp.
+
+Section tpreinst.
+  Context {lang : lang.t}.
+
+  (* TODO: this type probably does not need to be parametric in [lang.t]
+     The only meaningful instantation is [lang.cpp]
+   *)
+  Record tpreinst' : Set := TPreInst {
+    tpreinst_name : temp_name;
+    tpreinst_args : list (temp_arg' lang);
+  }.
+
+  #[global] Instance tpreinst'_inhabited : Inhabited tpreinst'.
+  Proof. solve_inhabited. Qed.
+
+  #[global] Instance tpreinst'_eq_dec : EqDecision tpreinst'.
+  Proof. solve_decision. Defined.
+End tpreinst.
+Add Printing Constructor tpreinst'.
+#[global] Arguments tpreinst' : clear implicits.
+#[global] Arguments TPreInst {_} _ & _ : assert.
+
+(** ** Template instances *)
+Section tinst.
+  #[local] Set Universe Polymorphism.
+  #[local] Set Polymorphic Inductive Cumulativity.
+  #[local] Unset Auto Template Polymorphism.
+  Universe uV.
+  Context {lang : lang.t} {V : Type@{uV}}.
+
+  Record tinst' : Type@{uV} := TInst {
+    tinst_params : list (temp_param' lang.temp);
+    tinst_args : list (temp_arg' lang);
+    tinst_value : V;
+  }.
+
+  #[global] Instance tinst'_inhabited `{!Inhabited V} : Inhabited tinst'.
+  Proof. solve_inhabited. Qed.
+
+  #[global] Instance tinst'_eq_dec
+      `{!EqDecision V} :
+    EqDecision tinst'.
+  Proof. solve_decision. Defined.
+End tinst.
+Add Printing Constructor tinst'.
+#[global] Arguments tinst' : clear implicits.
+#[global] Arguments TInst {_ _} _ _ & _ : assert.
+
+Notation temp_param := (temp_param' lang.cpp).
+Notation temp_arg := (temp_arg' lang.cpp).
